Nemonuri/HasHUnion/SetLike.lean
@@ -6,6 +6,13 @@ public import Nemonuri.HasHUnion.Basic
 
 set_option autoImplicit false
 
+namespace Nemonuri
+
+abbrev DecidableSetLikeMem (S E: Type*) [SetLike S E] : Type _ := (s: S) → (e: E) → Decidable (e ∈ s)
+
+end Nemonuri
+
+
 namespace Nemonuri.HasHUnion
 
 section EmbedSetAt
@@ -13,129 +20,489 @@ section EmbedSetAt
 universe u1 u2
 variable {L1 L2: Type u1} [HasHUnion.{u1, u2} L1 L2]
 
-def RightSet (L1 L2: Type u1) [HasHUnion.{u1, u2} L1 L2] : Type _ := Set (R L1 L2)
+def leftSetAt (lb: Label) (ls1: Set L1) (ls2: Set L2) : Set (LeftTypeAt L1 L2 lb) :=
+  lb.casesOn (motive := fun lb0 => Set (LeftTypeAt L1 L2 lb0)) ls1 ls2
 
-def embedSetAt (lb: Label) (s: Set (LeftTypeAt L1 L2 lb)) : RightSet L1 L2 := s.image (embedAt L1 L2 lb)
 
-theorem embedSetAt_injective {lb: Label} : Function.Injective (embedSetAt lb: Set (LeftTypeAt L1 L2 lb) → RightSet L1 L2) := by
-  intro s1 s2 lm1
-  dsimp [embedSetAt, RightSet] at lm1
-  simp [Set.ext_iff] at lm1 ⊢
-  intro lv
-  specialize lm1 (embedAt L1 L2 lb lv)
-  simp [embedAt_injective.eq_iff] at lm1
-  exact lm1
+def RightSet (L1 L2: Type u1) [HasHUnion.{u1, u2} L1 L2] : Type _ := Set (HUnionElemAt L1 L2)
 
-theorem embedSetAt_injective_at (lb: Label) : Function.Injective (embedSetAt lb: Set (LeftTypeAt L1 L2 lb) → RightSet L1 L2) := embedSetAt_injective
+
+namespace HUnionElemAt
+
+inductive IsInUnion (ls1: Set L1) (ls2: Set L2) (rv: HUnionElemAt L1 L2) : Prop where --(HUnionElemAt L1 L2) →
+  | fst (lv: L1) (req1: lv ∈ ls1) (req2: embedAt L1 L2 .fst lv = rv.val) --: IsInUnion ls1 ls2 (.pureFst L1 L2 lv)
+  | snd (lv: L2) (req1: lv ∈ ls2) (req2: embedAt L1 L2 .snd lv = rv.val) --: IsInUnion ls1 ls2 (.pureSnd L1 L2 lv)
+
+theorem isInUnion_iff_exists {ls1: Set L1} {ls2: Set L2} {rv: HUnionElemAt L1 L2}
+  : (IsInUnion ls1 ls2 rv) ↔ (∃(lb: Label), ∃(lv: LeftTypeAt L1 L2 lb), lv ∈ leftSetAt lb ls1 ls2 ∧ embedAt L1 L2 lb lv = rv.val) := by
+  constructor
+  · rintro lm1
+    rcases lm1 with ⟨lv, lm1, lm2⟩ | ⟨lv, lm1, lm2⟩
+    · exists .fst
+      exists lv
+    · exists .snd
+      exists lv
+  · rintro ⟨lb, lv, lm1, lm2⟩
+    rcases lb
+    · exact .fst lv lm1 lm2
+    · exact .snd lv lm1 lm2
+
+def decideIsInUnion [DecidableEmbedRange L1 L2] (ls1: Set L1) (ls2: Set L2) [DecidablePred (· ∈ ls1)] [DecidablePred (· ∈ ls2)] (rv: HUnionElemAt L1 L2) : Bool :=
+  rv.recDiffInter₂
+    (fun lb lv _ => lb.casesOn (fun lv0 => decide (lv0 ∈ ls1)) (fun lv0 => decide (lv0 ∈ ls2)) <| lv)
+    (fun rv lm1 =>
+      (decide (HasHUnion.liftAt L1 L2 rv .fst (lm1 .fst) ∈ ls1)) || (decide (HasHUnion.liftAt L1 L2 rv .snd (lm1 .snd) ∈ ls2)))
+    --(fun rv0 => decide (rv0.lift ∈ ls1))
+    --(fun rv0 => decide (rv0.lift ∈ ls2))
+    --(fun rv0 => decide (rv0.liftAt .fst ∈ ls1) || decide (rv0.liftAt .snd ∈ ls2))
+
+
+theorem decideIsInUnion_eq_true_iff_in_union
+  [DecidableEmbedRange L1 L2] {ls1: Set L1} {ls2: Set L2} [DecidablePred (· ∈ ls1)] [DecidablePred (· ∈ ls2)] {rv: HUnionElemAt L1 L2}
+  : (decideIsInUnion ls1 ls2 rv) ↔ (IsInUnion ls1 ls2 rv) := by
+  cases rv using recDiffInter₂
+  · rename_i lb lv lm1
+    dsimp [decideIsInUnion]
+    rw [recDiffInter₂_diff lm1]
+    rcases lb
+    · simp
+      constructor
+      · intro lm3
+        refine .fst lv lm3 ?_
+        exact pureAt_val_eq_embedAt.symm
+      · intro lm3
+        rcases lm3 with ⟨lv2, lm3, lm4⟩ | ⟨lv2, lm3, lm4⟩
+        · simp [pureAt_val_eq_embedAt, embedAt_injective.eq_iff] at lm4
+          subst lm4
+          exact lm3
+        · simp [pureAt_val_eq_embedAt] at lm4
+          simp [← lm4] at lm1
+    · simp
+      constructor
+      · intro lm3
+        refine .snd lv lm3 ?_
+        exact pureAt_val_eq_embedAt.symm
+      · intro lm3
+        rcases lm3 with ⟨lv2, lm3, lm4⟩ | ⟨lv2, lm3, lm4⟩
+        · simp [pureAt_val_eq_embedAt] at lm4
+          simp [← lm4] at lm1
+        · simp [pureAt_val_eq_embedAt, embedAt_injective.eq_iff] at lm4
+          subst lm4
+          exact lm3
+  · rename_i rv lm1
+    dsimp [decideIsInUnion]
+    rw [recDiffInter₂_inter lm1]
+    simp
+    constructor
+    · intro lm2
+      rcases lm2 with lm2 | lm2
+      · refine .fst (HasHUnion.liftAt L1 L2 rv .fst (lm1 .fst)) ?_ ?_
+        · exact lm2
+        · simp [liftAt_embedAt_eq, ofInter, ofRightType_def]
+      · refine .snd (HasHUnion.liftAt L1 L2 rv .snd (lm1 .snd)) ?_ ?_
+        · exact lm2
+        · simp [liftAt_embedAt_eq, ofInter, ofRightType_def]
+    · intro lm3
+      rcases lm3 with ⟨lv2, lm3, lm4⟩ | ⟨lv2, lm3, lm4⟩ <;> (
+        dsimp [ofInter, ofRightType_def] at lm4
+        rewrite [Eq.comm] at lm4
+        subst lm4
+        simp [embedAt_liftAt_eq] )
+      · exact Or.inl lm3
+      · exact Or.inr lm3
+
+instance decidableIsInUnion [DecidableEmbedRange L1 L2] {ls1: Set L1} {ls2: Set L2} [DecidablePred (· ∈ ls1)] [DecidablePred (· ∈ ls2)] {rv: HUnionElemAt L1 L2} : Decidable (IsInUnion ls1 ls2 rv) :=
+  decidable_of_iff (decideIsInUnion ls1 ls2 rv = .true) decideIsInUnion_eq_true_iff_in_union
+
+
+end HUnionElemAt
 
 namespace RightSet
 
-def ofSet (s: Set (R L1 L2)) : RightSet L1 L2 := s
+def ofHUnionSet (s: Set (HUnionElemAt L1 L2)) : RightSet L1 L2 := s
 
-def toSet (rs: RightSet L1 L2) : Set (R L1 L2) := rs
+def toHUnionSet (rs: RightSet L1 L2) : Set (HUnionElemAt L1 L2) := rs
 
 instance toUnion : Union (RightSet L1 L2) where
-  union rs1 rs2 := ofSet (rs1.toSet ∪ rs2.toSet)
+  union rs1 rs2 := ofHUnionSet (rs1.toHUnionSet ∪ rs2.toHUnionSet)
 
 @[defeq]
-theorem union_def {rs1 rs2: RightSet L1 L2} : (rs1 ∪ rs2) = ofSet (rs1.toSet ∪ rs2.toSet) := rfl
+theorem union_def {rs1 rs2: RightSet L1 L2} : (rs1 ∪ rs2) = ofHUnionSet (rs1.toHUnionSet ∪ rs2.toHUnionSet) := rfl
 
-instance toMembership : Membership (R L1 L2) (RightSet L1 L2) where
-  mem rs re := re ∈ rs.toSet
+instance toMembership : Membership (HUnionElemAt L1 L2) (RightSet L1 L2) where
+  mem rs re := re ∈ rs.toHUnionSet
 
 @[defeq]
-theorem mem_def {rs: RightSet L1 L2} {re: R L1 L2} : (re ∈ rs) = (re ∈ rs.toSet) := rfl
+theorem mem_def {rs: RightSet L1 L2} {re: HUnionElemAt L1 L2} : (re ∈ rs) = (re ∈ rs.toHUnionSet) := rfl
+
+def pureAt (lb: Label) (s: Set (LeftTypeAt L1 L2 lb)) : RightSet L1 L2 := s.image (HUnionElemAt.pureAt L1 L2 lb)
+
+
+theorem pureAt_injective {lb: Label} : Function.Injective (pureAt lb: Set (LeftTypeAt L1 L2 lb) → RightSet L1 L2) := by
+  intro s1 s2 lm1
+  dsimp [pureAt, RightSet] at lm1
+  simp [Set.ext_iff] at lm1 ⊢
+  intro lv
+  specialize lm1 (HUnionElemAt.pureAt L1 L2 lb lv)
+  simp [HUnionElemAt.pureAt_eq_embedAt_mk, embedAt_injective.eq_iff, hunionSetUnivAt_mem_iff_embedRangeAt_mem] at lm1
+  exact lm1 lb EmbedRangeAt.mem_self
+
+theorem pureAt_injective_at (lb: Label) : Function.Injective (pureAt lb: Set (LeftTypeAt L1 L2 lb) → RightSet L1 L2) := pureAt_injective
+
+theorem pureAt_pureAt_mem_iff_mem {lb: Label} {s: Set (LeftTypeAt L1 L2 lb)} {lv: LeftTypeAt L1 L2 lb} --{re: HUnionElemAt L1 L2}
+  : (HUnionElemAt.pureAt L1 L2 lb lv ∈ (pureAt lb s)) ↔ (lv ∈ s) := by
+  dsimp [mem_def, HUnionElemAt.pureAt_eq_embedAt_mk, toHUnionSet]
+  constructor
+  · intro lm1
+    simp [pureAt, HUnionElemAt.pureAt_eq_embedAt_mk, embedAt_injective.eq_iff] at lm1
+    exact lm1
+  · intro lm1
+    simp [pureAt, HUnionElemAt.pureAt_eq_embedAt_mk, embedAt_injective.eq_iff]
+    exact lm1
+
+/-
+theorem pureAt_ofRightType_mem_iff_liftAt_mem {lb: Label} {s: Set (LeftTypeAt L1 L2 lb)} {rv: R L1 L2} (req: rv ∈ EmbedRangeAt L1 L2 lb)
+  : (HUnionElemAt.ofRightType rv (hunionSetUnivAt_mem_of_embedRangeAt_mem req) ∈ (pureAt lb s)) ↔ (liftAt L1 L2 rv lb req ∈ s) := by
+  conv =>
+    rhs
+    rw [← pureAt_pureAt_mem_iff_mem, HUnionElemAt.pureAt_eq_embedAt_mk]
+    simp only [liftAt_embedAt_eq]
+    rw [← HUnionElemAt.ofRightType_def]
+-/
+
+theorem pureAt_mem_iff {lb: Label} {s: Set (LeftTypeAt L1 L2 lb)} {rv: HUnionElemAt L1 L2}
+  : (rv ∈ (pureAt lb s)) ↔ (∃(req: rv.val ∈ EmbedRangeAt L1 L2 lb), (liftAt L1 L2 rv.val lb req) ∈ s) := by
+  dsimp [mem_def, toHUnionSet]
+  simp [pureAt, EmbedRangeAt.exists_embedAt_iff]
+  constructor
+  · rintro ⟨lv, lm1, lm2⟩
+    rewrite [Eq.comm] at lm2
+    subst lm2
+    simp [HUnionElemAt.pureAt_val_eq_embedAt, embedAt_liftAt_eq]
+    exact lm1
+  · rintro ⟨⟨lv, lm1⟩, lm2⟩
+    exists lv
+    simp [← lm1, embedAt_liftAt_eq] at lm2
+    refine ⟨lm2, ?_⟩
+    simp [HUnionElemAt.pureAt_eq_embedAt_mk, lm1]
+
+
+/-
+  constructor
+  · intro lm1
+    simp [pureAt] at lm1
+-/
+    --rewrite [Set.mem_image]
+
+
+def hunion (ls1: Set L1) (ls2: Set L2) : RightSet L1 L2 := ofHUnionSet { rv | HUnionElemAt.IsInUnion ls1 ls2 rv } --(pureAt .fst ls1) ∪ (pureAt .snd ls2)
+
+/-
+theorem hunion_mem_iff_exists {ls1: Set L1} {ls2: Set L2} {rv: HUnionElemAt L1 L2}
+  : (rv ∈ hunion ls1 ls2) ↔ (∃(lb: Label), ∃(req: rv.val ∈ EmbedRangeAt L1 L2 lb), (liftAt L1 L2 rv lb req) ∈ (leftSetAt lb ls1 ls2)) := by
+  dsimp [hunion, union_def, ofHUnionSet, toHUnionSet, mem_def]
+  constructor
+  · intro lm1
+    rewrite [Set.mem_union] at lm1
+    rcases lm1 with lm1 | lm1
+    · exists Label.fst
+      dsimp [leftSetAt]
+      exact pureAt_mem_iff.mp lm1
+    · exists Label.snd
+      dsimp [leftSetAt]
+      exact pureAt_mem_iff.mp lm1
+  · rintro ⟨lb, lm1⟩
+    rewrite [← pureAt_mem_iff] at lm1
+    rw [Set.mem_union]
+    rcases lb <;> dsimp [leftSetAt] at lm1
+    · exact Or.inl lm1
+    · exact Or.inr lm1
+-/
+
 
 end RightSet
+
+
 
 end EmbedSetAt
 
 universe u1 u2 u3
 variable {LS1 LS2: Type u1} {L1 L2: Type u2} [SetLike LS1 L1] [SetLike LS2 L2] [HasHUnion.{u2, u3} L1 L2]
 
-namespace RightSet
-
-def ofSetLikeHUnion (ls1: LS1) (ls2: LS2) : RightSet L1 L2 := (embedSetAt .fst (ls1: Set L1)) ∪ (embedSetAt .snd (ls2: Set L2))
-
-structure SetLikeHUnionMemDecidableProd (LS1 LS2: Type u1) (L1 L2: Type u2) [SetLike LS1 L1] [SetLike LS2 L2] [HasHUnion.{u2, u3} L1 L2] where
+structure SetLikeProd (LS1 LS2: Type u1) (L1 L2: Type u2) [SetLike LS1 L1] [SetLike LS2 L2] [HasHUnion.{u2, u3} L1 L2] where
   fst: LS1
   snd: LS2
-  toDecidableMem (elemR: R L1 L2) : Decidable (elemR ∈ ofSetLikeHUnion fst snd)
 
 
-namespace SetLikeHUnionMemDecidableProd
+
+namespace SetLikeProd
+
+def decideMem [DecidableEmbedRange L1 L2] (s: SetLikeProd LS1 LS2 L1 L2) [DecidablePred (· ∈ s.fst)] [DecidablePred (· ∈ s.snd)] (rv: HUnionElemAt L1 L2) : Bool :=
+  HUnionElemAt.decideIsInUnion s.fst s.snd rv
+
+theorem decideMem_eq_true_iff_in_union
+  [DecidableEmbedRange L1 L2] {s: SetLikeProd LS1 LS2 L1 L2}
+  [DecidablePred (· ∈ s.fst)] [DecidablePred (· ∈ s.snd)] {rv: HUnionElemAt L1 L2}
+  : (s.decideMem rv = .true) ↔ HUnionElemAt.IsInUnion s.fst s.snd rv := by
+  dsimp [decideMem]
+  simp [HUnionElemAt.decideIsInUnion_eq_true_iff_in_union]
+
+open HUnionElemAt
+
+def AreUnionEquiv (p1 p2: SetLikeProd LS1 LS2 L1 L2) : Prop := ∀⦃rv: HUnionElemAt L1 L2⦄, IsInUnion p1.fst p1.snd rv ↔ IsInUnion p2.fst p2.snd rv
+
+
+namespace AreUnionEquiv
+
+theorem mk {p1 p2: SetLikeProd LS1 LS2 L1 L2} (req: ∀(rv: HUnionElemAt L1 L2), IsInUnion p1.fst p1.snd rv ↔ IsInUnion p2.fst p2.snd rv) : AreUnionEquiv p1 p2 := req
+
+theorem equivalence : Equivalence (AreUnionEquiv: SetLikeProd LS1 LS2 L1 L2 → SetLikeProd LS1 LS2 L1 L2 → Prop) where
+  refl x := by intro x; rfl
+  symm := by
+    intro x y lm1 rv
+    specialize @lm1 rv
+    exact lm1.symm
+  trans := by
+    intro x y z lm1 lm2 rv
+    specialize @lm1 rv
+    specialize @lm2 rv
+    exact Iff.trans lm1 lm2
+
+
+@[reducible]
+def setoidOf (LS1 LS2: Type u1) (L1 L2: Type u2) [SetLike LS1 L1] [SetLike LS2 L2] [HasHUnion.{u2, u3} L1 L2] : Setoid (SetLikeProd LS1 LS2 L1 L2) where
+  r p1 p2 := AreUnionEquiv p1 p2
+  iseqv := equivalence
+
+
+--def decideOf (p1 p2: SetLikeProd LS1 LS2 L1 L2) : Bool := decide (IsInUnion p1.fst p1.snd )
+
+
+
+end AreUnionEquiv
+
+end SetLikeProd
+
+def SetLikeUnion (LS1 LS2: Type u1) (L1 L2: Type u2) [SetLike LS1 L1] [SetLike LS2 L2] [HasHUnion.{u2, u3} L1 L2] : Type _ := Quotient (SetLikeProd.AreUnionEquiv.setoidOf LS1 LS2 L1 L2)
+
+namespace SetLikeUnion
+
+def mk (sp: SetLikeProd LS1 LS2 L1 L2) : SetLikeUnion LS1 LS2 L1 L2 := Quotient.mk _ sp
+
+@[elab_as_elim]
+theorem ind
+  {motive: SetLikeUnion LS1 LS2 L1 L2 → Prop}
+  (h: (sp: SetLikeProd LS1 LS2 L1 L2) → motive (.mk sp))
+  (t: SetLikeUnion LS1 LS2 L1 L2)
+  : motive t := by
+  cases t using Quotient.ind
+  rename_i sp
+  specialize h sp
+  dsimp [mk] at h
+  exact h
+
+def liftOn
+  {β: Sort*} (su: SetLikeUnion LS1 LS2 L1 L2)
+  (f: SetLikeProd LS1 LS2 L1 L2 → β)
+  (c: ∀(sp1 sp2: SetLikeProd LS1 LS2 L1 L2), sp1.AreUnionEquiv sp2 → f sp1 = f sp2)
+  : β :=
+  Quotient.liftOn su f c
+
+theorem mk_eq_iff {sp1 sp2: SetLikeProd LS1 LS2 L1 L2} : (mk sp1 = mk sp2) ↔ sp1.AreUnionEquiv sp2 := by
+  dsimp [mk]
+  constructor
+  · intro lm1
+    exact Quotient.eq_iff_equiv.mp lm1
+  · intro lm1
+    exact Quotient.sound lm1
+
+
+variable [DecidableSetLikeMem LS1 L1] [DecidableSetLikeMem LS2 L2] [DecidableEmbedRange L1 L2]
+
+
+def decideMem (s: SetLikeUnion LS1 LS2 L1 L2) (rv: HUnionElemAt L1 L2) : Bool :=
+  s.liftOn (fun sp => sp.decideMem rv) (by
+    intro sp1 sp2 lm1
+    dsimp [SetLikeProd.decideMem]
+    rw [Bool.eq_iff_iff]
+    simp [HUnionElemAt.decideIsInUnion_eq_true_iff_in_union]
+    exact @lm1 rv)
+
+theorem decideMem_eq_true_iff {s: SetLikeProd LS1 LS2 L1 L2} {rv: HUnionElemAt L1 L2}
+  : (decideMem (mk s) rv = .true) ↔ HUnionElemAt.IsInUnion s.fst s.snd rv := by
+  dsimp [decideMem]
+  simp [← SetLikeProd.decideMem_eq_true_iff_in_union, mk]
+  dsimp [liftOn]
+  refine Quotient.liftOn_mk _ _ s
+
+
+def toRightSet (s: SetLikeUnion LS1 LS2 L1 L2) : Set (HUnionElemAt L1 L2) := { rv | s.decideMem rv = .true }
+
+
+theorem toRightSet_injective : Function.Injective (toRightSet: SetLikeUnion LS1 LS2 L1 L2 → Set (HUnionElemAt L1 L2)) := by
+  intro s1 s2 lm1
+  cases s1 using SetLikeUnion.ind
+  cases s2 using SetLikeUnion.ind
+  rename_i sp1 sp2
+  simp [- Subtype.forall, Set.ext_iff, toRightSet, decideMem_eq_true_iff] at lm1
+  rw [mk_eq_iff]
+  intro rv
+  exact lm1 rv
+
+instance toSetLike : SetLike (SetLikeUnion LS1 LS2 L1 L2) (HUnionElemAt L1 L2) where
+  coe x := x.toRightSet
+  coe_injective := toRightSet_injective
+
+
+end SetLikeUnion
+
+
+class HasSetLike.{u4} (L1 L2 : Type u2) [HasHUnion.{u2, u3} L1 L2] [DecidableEmbedRange L1 L2] where
+  LS1: Type u1
+  leftSetLike1: SetLike LS1 L1
+  decidableLeftSetLikeMem1: DecidableSetLikeMem LS1 L1
+  LS2: Type u1
+  leftSetLike2: SetLike LS2 L2
+  decidableLeftSetLikeMem2: DecidableSetLikeMem LS2 L2
+  leftSetHasHUnion: HasHUnion.{u1, u4} LS1 LS2
+  protected coe: (R LS1 LS2) → SetLikeUnion LS1 LS2 L1 L2
+  coe_injective: Function.Injective coe
+
+attribute [reducible, instance] HasSetLike.leftSetLike1 HasSetLike.leftSetLike2 HasSetLike.leftSetHasHUnion
+                                HasSetLike.decidableLeftSetLikeMem1 HasSetLike.decidableLeftSetLikeMem2
+attribute [coe] HasSetLike.coe
+
+namespace HasSetLike
+
+universe u4
+
+abbrev RS (L1 L2 : Type u2) [HasHUnion.{u2, u3} L1 L2] [DecidableEmbedRange L1 L2] [HasSetLike.{u1, u2, u3, u4} L1 L2] : Type _ := (HasSetLike.leftSetHasHUnion: HasHUnion (HasSetLike.LS1 L1 L2) (HasSetLike.LS2 L1 L2)).R
+
+abbrev SetLikeUnionType (L1 L2 : Type u2) [HasHUnion.{u2, u3} L1 L2] [DecidableEmbedRange L1 L2] [HasSetLike.{u1, u2, u3, u4} L1 L2] : Type _ := SetLikeUnion (HasSetLike.LS1 L1 L2) (HasSetLike.LS2 L1 L2) L1 L2
+
+variable [DecidableEmbedRange L1 L2] [HasSetLike.{u1, u2, u3, u4} L1 L2]
+
+instance : CoeOut (RS L1 L2) (SetLikeUnionType L1 L2) where
+  coe rs := HasSetLike.coe rs
+
+
+instance toSetLike : SetLike (RS L1 L2) (HUnionElemAt L1 L2) where
+  coe rs := ((rs: SetLikeUnionType L1 L2): Set (HUnionElemAt L1 L2))
+  coe_injective := SetLike.coe_injective.comp HasSetLike.coe_injective
+
+
+
+
+
+end HasSetLike
+
+/-
+namespace RightSet
+
+namespace HUnionSetLikeProd
 
 variable [DecidableEmbedRange L1 L2]
 
 open DecidableEmbedRange
 
-def decideMem (ls1: LS1) (ls2: LS2) [DecidablePred (· ∈ ls1)] [DecidablePred (· ∈ ls2)] (er: R L1 L2) : Bool := --Decidable (er ∈ ofSetLikeHUnion ls1 ls2)
-  let loc1 (_: Unit) : Bool :=
-    if lm1_1: isInEmbedRangeAt L1 L2 er .snd = .true then
-      let lv : L2 := liftAt L1 L2 er .snd (isInEmbedRangeAt_eq_true_iff.mp lm1_1)
-      decide (lv ∈ ls2)
-    else
-      .false
-  if lm1: isInEmbedRangeAt L1 L2 er .fst = .true then
-    let lv : L1 := liftAt L1 L2 er .fst (isInEmbedRangeAt_eq_true_iff.mp lm1)
-    if decide (lv ∈ ls1) = .true then .true else loc1 ()
-  else
-    loc1 ()
 
-theorem decideMem_iff_ofSetLikeHUnion_mem {ls1: LS1} {ls2: LS2} [DecidablePred (· ∈ ls1)] [DecidablePred (· ∈ ls2)] {er: R L1 L2}
-  : (decideMem ls1 ls2 er = .true) ↔ (er ∈ ofSetLikeHUnion ls1 ls2) := by
-  dsimp [ofSetLikeHUnion, union_def, toSet, ofSet, mem_def]
-  simp [embedSetAt]
-  constructor
-  · intro lm1
-    simp [decideMem] at lm1
-    by_cases lm2: isInEmbedRangeAt L1 L2 er .fst = .true
-    · simp [lm2] at lm1
-      obtain ⟨lv, lm3⟩ := isInEmbedRangeAt_eq_true_iff.mp lm2 |> EmbedRangeAt.exists_embedAt_iff.mp
-      rewrite [Eq.comm] at lm3
-      subst lm3
-      simp [embedAt_liftAt_eq] at lm1
-      rcases lm1 with lm1 | lm1
-      · refine Or.inl ?_
-        exists lv
-      · refine Or.inr ?_
-        rcases lm1 with ⟨lm1, lm3⟩
-        obtain ⟨lv2, lm4⟩ := isInEmbedRangeAt_eq_true_iff.mp lm1 |> EmbedRangeAt.exists_embedAt_iff.mp
-        exists lv2
-        simp [lm4]
-        simp [← lm4, embedAt_liftAt_eq] at lm3
-        exact lm3
-    · simp at lm2
-      simp [lm2] at lm1
-      rcases lm1 with ⟨lm1, lm3⟩
-      obtain ⟨lv2, lm4⟩ := isInEmbedRangeAt_eq_true_iff.mp lm1 |> EmbedRangeAt.exists_embedAt_iff.mp
-      refine Or.inr ?_
-      rewrite [Eq.comm] at lm4
-      subst lm4
-      simp [embedAt_liftAt_eq] at lm3
-      exists lv2
-  · intro lm1
-    rcases lm1 with lm1 | lm1 <;> (rcases lm1 with ⟨lv, lm1, lm2⟩)
-    · rewrite [Eq.comm] at lm2
-      subst lm2
-      simp [decideMem, isInEmbedRangeAt_eq_true_iff, embedAt_liftAt_eq]
-      exact Or.inl lm1
-    · rewrite [Eq.comm] at lm2
-      subst lm2
-      simp [decideMem, isInEmbedRangeAt_eq_true_iff, embedAt_liftAt_eq, lm1]
+def decideMem (ls1: LS1) (ls2: LS2) [DecidablePred (· ∈ ls1)] [DecidablePred (· ∈ ls2)] (rv: HUnionElemAt L1 L2) : Bool := --Decidable (er ∈ ofSetLikeHUnion ls1 ls2)
+  rv.recDiffInter
+    (fun rv0 => decide (rv0.lift ∈ ls1))
+    (fun rv0 => decide (rv0.lift ∈ ls2))
+    (fun rv0 => decide (rv0.liftAt .fst ∈ ls1) || decide (rv0.liftAt .snd ∈ ls2))
+
+theorem decideMem_eq_true_iff_hunionSetLike_mem {ls1: LS1} {ls2: LS2} [DecidablePred (· ∈ ls1)] [DecidablePred (· ∈ ls2)] {rv: HUnionElemAt L1 L2}
+  : (decideMem ls1 ls2 rv = .true) ↔ (rv ∈ hunionSetLike ls1 ls2) := by
+  dsimp [hunionSetLike, mem_def, toHUnionSet, hunion, union_def, ofHUnionSet]
+  simp only [Set.mem_union]
+  dsimp [decideMem]
+  cases rv using HUnionElemAt.recDiffInter <;> rename_i rv
+  · simp
+    rcases rv with ⟨rv, lm1⟩
+    simp [hdiffSetUnivAt_mem_iff_embedRangAt_mem, EmbedRangeAt.exists_embedAt_iff] at lm1
+    rcases lm1 with ⟨⟨lv, lm1⟩, lm2⟩
+    rewrite [Eq.comm] at lm1
+    subst lm1
+    dsimp [Label.toDual] at lm2
+    simp [HDiffElemAt.toUnion, pureAt, HUnionElemAt.pureAt_eq_embedAt_mk, embedAt_injective.eq_iff]
+    simp [HDiffElemAt.lift, embedAt_liftAt_eq]
+    intro x lm3 lm4
+    exact lm2 x lm4 |>.elim
+  · simp
+    rcases rv with ⟨rv, lm1⟩
+    simp [hdiffSetUnivAt_mem_iff_embedRangAt_mem, EmbedRangeAt.exists_embedAt_iff] at lm1
+    rcases lm1 with ⟨⟨lv, lm1⟩, lm2⟩
+    rewrite [Eq.comm] at lm1
+    subst lm1
+    dsimp [Label.toDual] at lm2
+    simp [HDiffElemAt.toUnion, pureAt, HUnionElemAt.pureAt_eq_embedAt_mk, embedAt_injective.eq_iff]
+    simp [HDiffElemAt.lift, embedAt_liftAt_eq]
+    intro x lm3 lm4
+    exact lm2 x lm4 |>.elim
+  · simp
+    rcases rv with ⟨rv, lm1⟩
+    simp [hinterSetUnivAt_mem_iff_embedRangeAt_mem, EmbedRangeAt.exists_embedAt_iff] at lm1
+    obtain ⟨lv, lm2⟩ := lm1 .fst
+    rewrite [Eq.comm] at lm2
+    subst lm2
+    obtain ⟨lv2, lm2⟩ := lm1 .snd
+    dsimp [HInterElemAt.liftAt]
+    conv => lhs; arg 2; simp only [← lm2]
+    simp [embedAt_liftAt_eq]
+    simp [pureAt, HUnionElemAt.pureAt_eq_embedAt_mk, HInterElemAt.toUnion]
+    conv => rhs; arg 2; simp only [← lm2]
+    simp [embedAt_injective.eq_iff]
 
 
-def ofDecidableMem (ls1: LS1) (ls2: LS2) [DecidablePred (· ∈ ls1)] [DecidablePred (· ∈ ls2)] : SetLikeHUnionMemDecidableProd LS1 LS2 L1 L2 where
+
+def ofDecidableMem (ls1: LS1) (ls2: LS2) [DecidablePred (· ∈ ls1)] [DecidablePred (· ∈ ls2)] : HUnionSetLikeProd LS1 LS2 L1 L2 where
   fst := ls1
   snd := ls2
-  toDecidableMem er := decidable_of_iff (decideMem ls1 ls2 er = .true) decideMem_iff_ofSetLikeHUnion_mem
+  toDecidableMem er := decidable_of_iff (decideMem ls1 ls2 er = .true) decideMem_eq_true_iff_hunionSetLike_mem
 
 
+def toRightSet (x: HUnionSetLikeProd LS1 LS2 L1 L2) : RightSet L1 L2 := ofHUnionSet { rv | (x.toDecidableMem rv).decide = .true }
+
+theorem toRightSet_injective : Function.Injective (toRightSet: HUnionSetLikeProd LS1 LS2 L1 L2 → RightSet L1 L2) := by
+  intro x1 x2 lm1
+  dsimp [toRightSet, ofHUnionSet] at lm1
+  simp at lm1
+  replace lm1 := Set.ext_iff.mp lm1
+  dsimp [hunionSetLike] at lm1
+  simp only [hunion_mem_iff_exists] at lm1
+  rcases x1 with ⟨fst1, snd1, tdm1⟩
+  rcases x2 with ⟨fst2, snd2, tdm2⟩
+  simp [- Subtype.forall] at lm1 ⊢
+  refine ⟨?_, ?_, ?_⟩
+  · simp only [SetLike.ext_iff]
+    intro lv
+    specialize lm1 (HUnionElemAt.pureAt L1 L2 .fst lv)
+    simp [HUnionElemAt.pureAt_val_eq_embedAt] at lm1
+    rcases lm1 with ⟨lm2, lm3⟩
+    simp at lm2 lm3
+    simp [Label.forall_iff_fst_and_snd, embedAt_liftAt_eq, leftSetAt] at lm2 lm3
+    simp [Label.exists_iff_fst_or_snd, embedAt_liftAt_eq] at lm2 lm3
+    rcases lm2 with ⟨lm2_1, lm2_2⟩
+    rcases lm3 with ⟨lm3_1, lm3_2⟩
+    constructor
+    · clear lm3_1 lm3_2
+      intro lm1
+      simp [lm1] at lm2_1 --lm3_1 lm3_2; clear lm3_1 lm3_2
+      rcases lm2_1 with lm2_1 | lm2_1
+      · exact lm2_1
+      · rcases lm2_1 with ⟨lm4, lm5⟩
+        revert lm4
+        simp [EmbedRangeAt.exists_embedAt_iff]
+        intro lv2 lm4 lm5
+        simp [← lm4, embedAt_liftAt_eq] at lm5
+        clear lm2_2
 
 
-end SetLikeHUnionMemDecidableProd
+end HUnionSetLikeProd
 
 end RightSet
+-/
 
 --def RightSet : Type _ := Set (R L1 L2)
 
