Nemonuri/HasHUnion/Normalizer.lean
@@ -1,0 +1,63 @@
+module
+
+public import Mathlib.Order.Defs.Unbundled
+
+@[expose] public section
+
+set_option autoImplicit false
+
+namespace Nemonuri
+
+structure IsQuotientNormalizer {α: Type _} (s: Setoid α) (op: α → α) : Prop where
+  apply_eq (a1 a2: α) (req: s.r a1 a2) : (op a1) = (op a2)
+  apply_rel (a: α) : s.r a (op a)
+  --idem (a: α) : f (f a) = f a
+  --liftable (a1 a2: α) (req: s.r a1 a2) : f a1 = f a2
+
+@[defeq, simp]
+protected theorem setoid_hasEquiv_def {α: Type _} {s: Setoid α} {a1 a2: α} : (a1 ≈ a2) = (s.r a1 a2) := rfl
+
+namespace IsQuotientNormalizer
+
+variable {α: Type _} {s: Setoid α} {op: α → α}
+
+theorem idempotent (h: IsQuotientNormalizer s op) {a: α} : (op (op a)) = op a :=
+  (h.apply_eq a (op a) (h.apply_rel a)).symm
+
+theorem apply_eq_iff (h: IsQuotientNormalizer s op) {a1 a2: α} : ((op a1) = (op a2)) ↔ (s.r a1 a2) := by
+  have lm_tr : IsTrans _ s.r := s.iseqv.isTrans
+  constructor
+  · intro lm1
+    have lm2 := h.apply_rel (op a1)
+    conv at lm2 => arg 2; rw [lm1, h.idempotent]
+    simp
+    calc
+      s.r _ _ := h.apply_rel a1
+      s.r _ _ := lm2
+      s.r _ _ := h.apply_rel a2 |> s.symm
+  · exact h.apply_eq _ _
+
+theorem apply_eq_iff_at (h: IsQuotientNormalizer s op) (a1 a2: α) : ((op a1) = (op a2)) ↔ (s.r a1 a2) := h.apply_eq_iff
+
+def normalize (h: IsQuotientNormalizer s op) (q: Quotient s) : α := q.liftOn op (h.apply_eq)
+
+end IsQuotientNormalizer
+
+structure QuotientNormalizer {α: Type _} (s: Setoid α) where
+  op: α → α
+  valid: IsQuotientNormalizer s op
+
+
+namespace QuotientNormalizer
+
+variable {α: Type _} {s: Setoid α}
+
+def normalize (x: QuotientNormalizer s) (q: Quotient s) : α := x.valid.normalize q
+
+
+end QuotientNormalizer
+
+
+end Nemonuri
+
+end
